Add notations

theories/tests/add.v
@@ -1,4 +1,4 @@
-From iris_os.clang Require Import logic tactics.
+From iris_os.clang Require Import logic tactics notations.
 From iris.base_logic Require Import big_op.
 From iris_os.os Require Import spec interrupt.
 From iris.proofmode Require Import tactics.
@@ -9,8 +9,7 @@ Section example.
   Context `{clangG Σ, specG Σ} {N: namespace}.
 
   Parameter py: addr.
-  Parameter Y lock unlock: ident.
-  Definition y := Evalue (Vptr py).
+  Parameter x Y lock unlock: ident.
   Definition I := (∃ vy, py ↦ Vint32 vy @ Tint32 ∗ Y S↦ Vint32 vy)%I.  
 
   Definition invs (prio: nat) : iProp Σ :=
@@ -21,19 +20,12 @@ Section example.
 
   Context `{i: interrupt invs}.
 
-  Definition f_body (px: addr) : stmts :=
-    Sprim Pcli;;;
-    Sassign y (Ebinop oplus (Ederef y) (Ederef (Evalue (Vptr px)))) ;;;
-    Sassign (Evalue (Vptr px)) (Ederef y) ;;;
-    Sprim Psti;;;
-    Srete (Ederef (Evalue (Vptr px))).
-
-  Definition f_body' (x: ident) : stmts :=
-    Sprim Pcli;;;
-    Sassign y (Ebinop oplus (Ederef y) (Evar x)) ;;;
-    Sassign (Evar x) (Ederef y) ;;;
-    Sprim Psti;;;
-    Srete (Evar x).
+  Definition f_body : stmts :=
+    cli ;;
+    py <- !py + x ;;
+    x <- !py ;;
+    sti ;;
+    rete x.
 
   Definition f_rel (vx: int) (s: spec_state) (r: option val) (s': spec_state) :=
     ∃ vy:int, s !! Y = Some (Vint32 vy) ∧
@@ -42,21 +34,19 @@ Section example.
 
   Definition int_ctx := @int_ctx _ _ invs i.
 
-
-
-
   Lemma f_spec γ γp px vx Φ Φret:
     int_ctx N γ γp ∗ inv N spec_inv ∗ hpri invs γp 1 ∗
     px ↦ Vint32 vx @ Tint32 ∗ scode (SCrel (f_rel vx)) ∗
     (∀ v, px ↦ v @ Tint32 -∗ scode (SCdone (Some v)) -∗ hpri invs γp 1 -∗ Φret v)
-    ⊢ WP curs (f_body px) {{ Φ ; Φret }}.
+    ⊢ WP curs (subst_s x px f_body) {{ Φ ; Φret }}.
   Proof.
     iIntros "(#? & #? & Hp & Hx & Hsc & HΦret)".
+    simpl. destruct (decide (x = x))=>//.
     iApply wp_seq.
     iApply cli_spec.
     iFrame "#". iFrame.
     iIntros "HI Hp Hcl".
-    simpl. iDestruct "HI" as (vy) "[Hy HY]". iApply fupd_wp.
+    iDestruct "HI" as (vy) "[Hy HY]". iApply fupd_wp.
     (* Open invariant *)
     iInv N as ">Hspec" "Hclose".
     iDestruct (spec_update {[ Y := Vint32 vy ]} _ {[ Y := Vint32 (Int.add vx vy) ]}
@@ -66,9 +56,9 @@ Section example.
       iFrame "Hsc". 
       iPureIntro. apply spec_step_rel. unfold f_rel.
       exists vy. gmap_solve. }
+    (* close invariant *)
     iMod ("Hclose" with "[Hspec]"); first eauto. iModIntro.
     iApply wp_seq.
-    rewrite /example.y.
     wp_load.
     wp_load.
     wp_op.
@@ -88,8 +78,8 @@ Section example.
     by rewrite Int.add_commut.
   Qed.
   
-  Lemma f_spec' (p: program) (x: ident) γ γp f vx Φ Φret:
-    p f = Some (Tint32, [(x, Tint32)], f_body' x) →
+  Lemma f_spec' (p: program) γ γp f vx Φ Φret:
+    p f = Some (Tint32, [(x, Tint32)], f_body) →
     int_ctx N γ γp ∗ inv N spec_inv ∗ hpri invs γp 1 ∗
     scode (SCrel (f_rel vx)) ∗ (∀ v, scode (SCdone (Some v)) -∗ hpri invs γp 1 -∗ Φ)
     ⊢ WP curs (Scall f [Evalue (Vint32 vx)]) {{ _, Φ ; Φret }}.
@@ -100,8 +90,7 @@ Section example.
     iIntros (ls) "% Hls".
     destruct ls as [|a [|b ls]].
     - simpl. iDestruct "Hls" as "%"=>//.
-    - simpl. destruct (decide (x = x))=>//.
-      iDestruct "Hls" as "[Hx _]".
+    - iDestruct "Hls" as "[Hx _]".
       iApply f_spec. iFrame "#". iFrame.
       iIntros (v) "_ Hsc Hp".
       iApply ("HΦ" with "[Hsc]")=>//.
