theories/clang/notations.v
@@ -1,0 +1,39 @@
+From iris_os.clang Require Import lang.
+Set Default Proof Using "Type".
+
+Coercion Vint8 : int8 >-> val.
+Coercion Vint32 : int32 >-> val.
+Coercion Vptr : addr >-> val.
+
+(* Coercion App : expr >-> Funclass. *)
+Coercion of_val : val >-> expr.
+
+Coercion Evar : ident >-> expr.
+
+Notation "'void'" := Vvoid : val_scope.
+Notation "'null'" := Vnull : val_scope.
+Notation "! e" := (Ederef e%E) (at level 9, right associativity) : expr_scope.
+Notation "& e" := (Eaddrof e%E)
+  (at level 30, right associativity) : expr_scope.
+Notation "e1 + e2" := (Ebinop oplus e1%E e2%E)
+  (at level 50, left associativity) : expr_scope.
+Notation "e1 - e2" := (Ebinop ominus e1%E e2%E)
+  (at level 50, left associativity) : expr_scope.
+Notation "e 'as' t" := (Ecast e%E t)
+  (at level 50, left associativity) : expr_scope.
+
+Notation "e1 <- e2" := (Sassign e1%E e2%E) (at level 80) : stmts_scope.
+Notation "'if' ( e ) { s1 } 'else' { s2 }" := (Sif e%E s1%S s2%S)
+  (at level 200, e, s1, s2 at level 200) : stmts_scope.
+Notation "'while' ( e ) { s }" := (Swhile e%E s%S)
+  (at level 200, e, s at level 200) : stmts_scope.
+Notation "s1 ;; s2" := (Sseq s1%S s2%S)
+  (at level 100, s2 at level 200, format "s1  ;;  s2") : stmts_scope.
+Notation "'ret'" := Sret (at level 80): stmts_scope.
+Notation "'rete' e" := (Srete e%E) (at level 80): stmts_scope.
+Notation "f < e1 , e2 , .. , en >" := (Scall f (cons e1%E (cons e2%E .. (cons en%E nil) .. )))
+  (at level 80) : stmts_scope.
+
+Notation "'cli'" := (Sprim Pcli) (at level 80) : stmts_scope.
+Notation "'sti'" := (Sprim Psti) (at level 80) : stmts_scope.
+
